\begin{problem}
با داشتن
$\sum_{1}^{n}i = \frac{n(n + 1)}{2}$
و
$\sum_{1}^{n}i^2 = \frac{n(n + 1)(2n + 1}{6}$
پاسخ
$\sum_{1}^{n}i^3$
را به دست آورید.
    \problemsolution{
    \begin{center}
        \p
     از اتحاد توان چهارم استفاده می‌کنیم:
        \p
        $n^4 - (n - 1)^4 = 4n^3 - 6n^2 + 4n - 1$
        \p
        $(n - 1)^4 - (n - 2)^4 = 4(n - 1)^3 - 6(n - 1)^2 + 4(n - 1) - 1$
        \p
       	$\vdots$
       	\p
       	$3^4 - 2^4 = 4(3)^3 - 6(3)^2 + 4(3) - 1$
       	\p
       	$2^4 - 1^4 = 4(2)^3 - 6(2)^2 + 4(2) -1$
       	\p
        $\Downarrow$
        \p
        $n^4 - 1 = 4\sum_{i=2}^{n}i^3 - 6\sum_{i=2}^{n}i^2 + 4\sum_{i=2}^{n}i - (n - 1)$
        \p
        $\Rightarrow 4\sum_{i=2}^{n}i^3 = n^4 - 1 + 6(\frac{n(n+1)(2n+1)}{6} - 1)$
        \p
        $= n^4 + n(n + 1)(2n + 1) - 2n(n + 1) + n - 4$
        \p
        $\sum_{1}^{n}i^3 = (\frac{n(n + 1)}{2})^2$
    \end{center}
    }
\end{problem}