	\p
از اتحاد توان چهارم استفاده می‌کنیم:

        $$n^4 - (n - 1)^4 = 4n^3 - 6n^2 + 4n - 1$$
        $$(n - 1)^4 - (n - 2)^4 = 4(n - 1)^3 - 6(n - 1)^2 + 4(n - 1) - 1$$
       	$$\vdots$$
       	$$3^4 - 2^4 = 4(3)^3 - 6(3)^2 + 4(3) - 1$$
       	$$2^4 - 1^4 = 4(2)^3 - 6(2)^2 + 4(2) -1$$
        $$\Downarrow$$
        $$n^4 - 1 = 4\sum\limits_{i=2}^{n}i^3 - 6\sum\limits_{i=2}^{n}i^2 + 4\sum\limits_{i=2}^{n}i - (n - 1)$$
        $$\Rightarrow 4\sum\limits_{i=2}^{n}i^3 = n^4 - 1 + 6(\frac{n(n+1)(2n+1)}{6} - 1)$$
        $$= n^4 + n(n + 1)(2n + 1) - 2n(n + 1) + n - 4$$
        $$\sum\limits_{1}^{n}i^3 = (\frac{n(n + 1)}{2})^2$$