\begin{table}[!h]
    \caption{Useful Generating Functions}
    \label{tab:table1}
    \begin{tabular}{|c|c|}
    \hline
      \textbf{$G(x)$}&\textbf{$a_k$}\\
      \hline
      \vtop{\hbox{\strut $(1 + x)^n = \sum\limits_{k=0}^{n}C(n, k)x^k$}\hbox{\strut $= 1 + C(n, 1)x + C(n, 2)x^2 + \cdots + x^n$}}&$C(n, k)$\\
      \hline
      \vtop{\hbox{\strut $(1 + ax)^n = \sum\limits_{k=0}^{n}C(n, k)a^kx^k$}\hbox{\strut $= 1 + C(n, 1)ax + C(n, 2)a^2x^2 + \cdots + a^nx^n$}}&$C(n, k)a^k$\\
      \hline
      \vtop{\hbox{\strut $(1 + x^r)^n = \sum\limits_{k=0}^{n}C(n, k)x^{rk}$}\hbox{\strut $= 1 + C(n, 1)x^r + C(n, 2)x^{2r} + \cdots + x^{rn}$}}&$C(n, k/r) if r|k; 0 otherwise$\\
      \hline
      $\frac{1-x{n+1}}{1-x} = \sum\limits_{k=0}^{n}x^k = 1 + x + x^2 + \cdots + x^n$&$1 if k \leq n; 0 otherwise$\\
      \hline
      $\frac{1}{1-x} = \sum\limits_{k=0}^{\infty}x^k = 1 + x + x^2 + \cdots$&$1$\\
      \hline
      $\frac{1}{1-ax} = \sum\limits_{k=0}^{\infty}a^kx^k = 1 + ax + a^2x^2 + \cdots$&$a^k$\\
      \hline
       $\frac{1}{1-x^r} = \sum\limits_{k=0}^{\infty}x^{rk} = 1 + x^r + x^{2r} + \cdots$&$1 if r|k; 0 otherwise$\\
       \hline
       $\frac{1}{(1-x)^2} = \sum\limits_{k=0}^{\infty}(k+1)x^k = 1 + 2x + 3x^2 + \cdots$&$k + 1$\\
       \hline
       \vtop{\hbox{\strut $\frac{1}{(1-x)^n} = \sum\limits_{k=0}^{\infty}C(n + k - 1, k)x^k$}\hbox{\strut $= 1 + C(n, 1)x + C(n + 1, 2)x^2 + \cdots$}}&$C(n + k - 1, k) = C(n + k - 1, n - 1)$\\
       \hline
       \vtop{\hbox{\strut $\frac{1}{(1+x)^n} = \sum\limits_{k=0}^{\infty}C(n + k - 1, k)(-1)^kx^k$}\hbox{\strut $= 1 - C(n, 1)x + C(n + 1, 2)x^2 - \cdots$}}&$(-1)^kC(n + k - 1, k) = (-1)^kC(n + k - 1, n - 1)$\\
       \hline
       \vtop{\hbox{\strut $\frac{1}{(1-ax)^n} = \sum\limits_{k=0}^{\infty}C(n + k - 1, k)a^kx^k$}\hbox{\strut $= 1 + C(n, 1)ax + C(n + 1, 2)a^2x^2 + \cdots$}}&$C(n + k - 1, k)a^k = C(n + k - 1, n - 1)a^k$\\
       \hline
       $e^x = \sum\limits_{k=0}^{\infty}\frac{x^k}{k!} = 1 + x + \frac{x^2}{2!} + \frac{x^3}{3!} + \cdots$&$1/k!$\\
       \hline
       $ln(1 + x) = \sum\limits_{k=1}^{\infty}\frac{(-1)^k+1}{k}x^k = x - \frac{x^2}{2} + \frac{x^3}{3} - \frac{x^4}{4} + \cdots$&$(-1)^{k+1}/k$\\
    \end{tabular}
\end{table}

%	\englishblock{
%    \footnote{TABLE 1 Useful Generating Functions, 8 / Advanced Counting Techniques, Page 542, Discrete Mathematics and Its Applications, By Kenneth H. Rosen}
%	}