	\p
ابتدا جواب عمومی معادله‌ی همگن را به‌دست می‌آوریم:
$$r^3 - 6r^2 + 12r - 8 = 0$$
ریشه‌ی
$2$
از مرتبه‌ی
$3$
دارد.
\begin{enumerate}
\item
$$F(n) = n^2$$
$$F(n) = (n^2)(1^n)$$
$1$
ریشه‌ی معادله همگن نیست.
$$a_p = (p_2 \times n^2 + p_1 \times n + p_0)$$
\item
$$F(n) = 2^n$$
$$F(n) = (1) \times 2^n$$
$2$
ریشه‌ی معادله‌ی همگن از مرتبه‌ی
$3$
است.
$$a_p = n^3(p_0) \times 2^n$$
\item
$$F(n) = n \times 2^n$$
$$F(n) = (n) \times 2^n$$
$2$
ریشه‌ی معادله‌ی همگن از مرتبه‌ی
$3$
است.
$$a_p = n^3(p_1 \times n + p_0)\times2^n$$
\end{enumerate}